ironfleet/src/Dafny/Distributed/Impl/Lock/CmdLineParser.i.dfy
@@ -11,20 +11,17 @@ import opened Common__SeqIsUniqueDef_i
 
 function lock_config_parsing(args:seq<seq<byte>>) : seq<EndPoint>
 {
-  var (ok, endpoints) := parse_end_points(args);
-  if ok && |endpoints| > 0 && |endpoints| < 0x1_0000_0000_0000_0000 then
-    endpoints 
-  else 
-    []
+  parse_end_points(args).1
 }
 
 method ParseCmdLine(id:EndPoint, args:seq<seq<byte>>)
   returns (ok:bool, host_ids:seq<EndPoint>, my_index:uint64)
   requires EndPointIsValidPublicKey(id)
-  ensures ok ==> && 0 <= my_index as int < |host_ids|
+  ensures ok ==> && 0 <= my_index as int < |host_ids| < 0x1_0000_0000_0000_0000
                 && host_ids == lock_config_parsing(args)
                 && host_ids[my_index] == id
                 && SeqIsUnique(host_ids)
+                && (forall h :: h in host_ids ==> EndPointIsValidPublicKey(h))
 {
   ok := false;
 
